SSA/Experimental/Bits/Fast/Attr.lean
@@ -8,6 +8,5 @@ Authors: Siddharth Bhat
 -/
 import Lean
 
-/-- The simproc extension for the 'bv_automata' tactic, which rewrites the denotations of bitvectors into that of automata. -/
-register_simp_attr bv_automata_denote
-
+/-- Preprocessing steps for bv_automata_circuit. -/
+register_simp_attr bv_circuit_preprocess
